sys-init/WellFormed_SI.thy
@@ -24,6 +24,7 @@ imports
   "DSpecProofs.Kernel_DP"
   "SepDSpec.Separation_SD"
   "Lib.SimpStrategy"
+  "AInvs.Rights_AI"
 begin
 
 context begin interpretation Arch . (*FIXME: arch_split*)
@@ -135,24 +136,6 @@ where
          | PageTableCap _ _ ad     \<Rightarrow> ad \<noteq> None
          | PageDirectoryCap _ _ ad \<Rightarrow> ad \<noteq> None
          | _                       \<Rightarrow> False)"
-
-definition is_real_vm_cap :: "cdl_cap \<Rightarrow> bool"
-where
-  "is_real_vm_cap cap \<equiv>
-       (case cap of
-           FrameCap _ _ _ _ Real _     \<Rightarrow> True
-         | PageTableCap _ Real _     \<Rightarrow> True
-         | PageDirectoryCap _ Real _ \<Rightarrow> True
-         | _                         \<Rightarrow> False)"
-
-definition is_fake_vm_cap :: "cdl_cap \<Rightarrow> bool"
-where
-  "is_fake_vm_cap cap \<equiv>
-       (case cap of
-           FrameCap _ _ _ _ Fake _     \<Rightarrow> True
-         | PageTableCap _ Fake _     \<Rightarrow> True
-         | PageDirectoryCap _ Fake _ \<Rightarrow> True
-         | _                         \<Rightarrow> False)"
 
 (* Original caps must have default rights,
  * and original endpoint + notification caps must not be badged.
@@ -385,7 +368,7 @@ lemma well_formed_cap_cap_has_object_eq:
 
 lemma well_formed_cap_update_cap_objects [simp]:
   "is_untyped_cap cap
-  \<Longrightarrow> well_formed_cap (update_cap_objects x cap) = well_formed_cap cap"
+   \<Longrightarrow> well_formed_cap (update_cap_objects x cap) = well_formed_cap cap"
   apply (clarsimp simp: update_cap_object_def
                         update_cap_objects_def well_formed_cap_def)
   apply (cases cap, simp_all)
@@ -399,8 +382,7 @@ lemma well_formed_cap_update_cap_object [simp]:
 
 lemma cap_rights_inter_default_cap_rights:
   "\<lbrakk>well_formed_cap cap; cap_type cap = Some type\<rbrakk>
-  \<Longrightarrow> cap_rights (default_cap type ids sz dev) \<inter> cap_rights cap
-    = cap_rights cap"
+   \<Longrightarrow> cap_rights (default_cap type ids sz dev) \<inter> cap_rights cap = cap_rights cap"
   by (fastforce simp: well_formed_cap_def default_cap_def cap_type_def cap_rights_def
                       validate_vm_rights_def vm_read_write_def
                       vm_kernel_only_def vm_read_only_def
@@ -444,7 +426,7 @@ lemma well_formed_distinct_slots_of_list [elim!]:
 
 lemma well_formed_object_size_bits:
   "\<lbrakk>well_formed spec; cdl_objects spec obj_id = Some obj\<rbrakk>
-  \<Longrightarrow> object_size_bits (object_default_state obj) = object_size_bits obj"
+   \<Longrightarrow> object_size_bits (object_default_state obj) = object_size_bits obj"
   apply (clarsimp simp: well_formed_def)
   apply (erule_tac x=obj_id in allE)
   apply (clarsimp)
@@ -452,13 +434,13 @@ lemma well_formed_object_size_bits:
 
 lemma well_formed_well_formed_caps:
   "\<lbrakk>well_formed spec; cdl_objects spec obj_id = Some obj\<rbrakk>
-  \<Longrightarrow> well_formed_caps spec obj_id obj"
+   \<Longrightarrow> well_formed_caps spec obj_id obj"
   by (clarsimp simp: well_formed_def split: option.splits)
 
 lemma well_formed_well_formed_cap:
   "\<lbrakk>well_formed spec; cdl_objects spec obj_id = Some obj;
     object_slots obj slot = Some cap; cap \<noteq> NullCap\<rbrakk>
-  \<Longrightarrow> well_formed_cap cap"
+   \<Longrightarrow> well_formed_cap cap"
   apply (clarsimp simp: well_formed_def)
   apply (erule_tac x=obj_id in allE)
   apply (clarsimp simp: well_formed_caps_def)
@@ -475,13 +457,13 @@ lemma well_formed_well_formed_cap':
 
 lemma well_formed_well_formed_cap_to_object:
   "\<lbrakk>well_formed spec; cdl_objects spec obj_id = Some obj\<rbrakk>
-  \<Longrightarrow> well_formed_cap_to_object spec obj_id obj"
+   \<Longrightarrow> well_formed_cap_to_object spec obj_id obj"
   by (clarsimp simp: well_formed_def split: option.splits)
 
 lemma well_formed_well_formed_cap_to_real_object:
   "\<lbrakk>well_formed spec; cdl_objects spec obj_id = Some obj;
     object_slots obj slot = Some cap; cap \<noteq> NullCap\<rbrakk>
-  \<Longrightarrow> well_formed_cap_to_real_object spec cap"
+   \<Longrightarrow> well_formed_cap_to_real_object spec cap"
   apply (clarsimp simp: well_formed_def)
   apply (erule_tac x=obj_id in allE)
   apply (clarsimp simp: well_formed_caps_def)
@@ -499,7 +481,7 @@ lemma well_formed_well_formed_cap_to_real_object':
 lemma well_formed_well_formed_cap_types_match:
   "\<lbrakk>well_formed spec; cdl_objects spec obj_id = Some obj;
     object_slots obj slot = Some cap; cap \<noteq> NullCap\<rbrakk>
-  \<Longrightarrow> well_formed_cap_types_match spec cap"
+   \<Longrightarrow> well_formed_cap_types_match spec cap"
   apply (clarsimp simp: well_formed_def)
   apply (erule_tac x=obj_id in allE)
   apply (clarsimp simp: well_formed_caps_def)
@@ -516,7 +498,7 @@ lemma well_formed_well_formed_cap_types_match':
 
 lemma well_formed_cap_object_is_real:
   "\<lbrakk>well_formed spec; opt_cap slot spec = Some cap; cap_has_object cap\<rbrakk>
-  \<Longrightarrow> real_object_at (cap_object cap) spec"
+   \<Longrightarrow> real_object_at (cap_object cap) spec"
   apply (drule (1) well_formed_well_formed_cap_to_real_object', simp)
   apply (clarsimp simp: well_formed_cap_to_real_object_def)
   done
@@ -524,7 +506,7 @@ lemma well_formed_cap_object_is_real:
 lemma well_formed_types_match:
   "\<lbrakk>well_formed spec; opt_cap (obj_id, slot) spec = Some cap;
     cdl_objects spec (cap_object cap) = Some cap_obj; cap_has_object cap\<rbrakk>
-  \<Longrightarrow> Some (object_type cap_obj) = cap_type cap"
+   \<Longrightarrow> Some (object_type cap_obj) = cap_type cap"
   apply (frule cap_has_object_not_NullCap)
   apply (clarsimp simp: well_formed_def)
   apply (erule_tac x=obj_id in allE)
@@ -538,7 +520,7 @@ lemma well_formed_types_match:
 
 lemma well_formed_object_slots:
   "\<lbrakk>well_formed spec; cdl_objects spec obj_id = Some obj\<rbrakk>
-  \<Longrightarrow> dom (object_slots obj) = dom (object_slots (object_default_state obj))"
+   \<Longrightarrow> dom (object_slots obj) = dom (object_slots (object_default_state obj))"
   apply (clarsimp simp: well_formed_def)
   apply (erule allE [where x=obj_id])
   apply simp
@@ -547,8 +529,7 @@ lemma well_formed_object_slots:
 lemma well_formed_slot_object_size_bits:
   "\<lbrakk>well_formed spec; opt_cap (obj_id, slot) spec = Some cap;
     cdl_objects spec obj_id = Some obj; cnode_at obj_id spec\<rbrakk>
-  \<Longrightarrow> slot < 2 ^ object_size_bits obj"
-  apply (frule opt_cap_cdl_objects)
+   \<Longrightarrow> slot < 2 ^ object_size_bits obj"
   apply (clarsimp simp: well_formed_def object_at_def is_cnode_def)
   apply (erule_tac x=obj_id in allE)
   apply clarsimp
@@ -564,9 +545,26 @@ lemma well_formed_slot_object_size_bits:
   apply (clarsimp simp: object_slots_slots_of)
   done
 
+lemma well_formed_slot_object_size_bits_pt:
+  "\<lbrakk>well_formed spec; opt_cap (obj_id, slot) spec = Some cap;
+    pt_at obj_id spec; cdl_objects spec obj_id = Some obj\<rbrakk>
+   \<Longrightarrow> slot < 2 ^ object_size_bits obj"
+  apply (clarsimp simp: well_formed_def object_at_def is_pt_def)
+  apply (erule_tac x=obj_id in allE)
+  apply clarsimp
+  apply (subgoal_tac "slot \<in> dom (object_slots (object_default_state obj))")
+   apply (thin_tac "dom P = dom Q" for P Q)
+   apply (clarsimp simp: well_formed_caps_def)
+   apply (erule_tac x=slot in allE)
+   apply (clarsimp simp: object_default_state_def2 object_type_def has_slots_def
+                         default_tcb_def object_size_bits_def object_slots_def
+                         empty_cnode_def empty_cap_map_def pt_size_def pd_size_def
+                   split: cdl_object.splits if_split_asm)
+  by (fastforce intro: object_slots_opt_capI)
+
 lemma well_formed_cnode_object_size_bits:
   "\<lbrakk>well_formed spec; cnode_at obj_id spec; cdl_objects spec obj_id = Some obj\<rbrakk>
-  \<Longrightarrow> 0 < object_size_bits obj"
+   \<Longrightarrow> 0 < object_size_bits obj"
   apply (clarsimp simp: well_formed_def)
   apply (erule_tac x=obj_id in allE)
   apply (clarsimp simp: is_cnode_def object_at_def)
@@ -575,7 +573,7 @@ lemma well_formed_cnode_object_size_bits:
 lemma well_formed_cnode_object_size_bits_eq:
   "\<lbrakk>well_formed spec; opt_cap slot spec = Some cap;
     cdl_objects spec (cap_object cap) = Some obj; is_cnode_cap cap\<rbrakk>
-  \<Longrightarrow> object_size_bits obj = cnode_cap_size cap"
+   \<Longrightarrow> object_size_bits obj = cnode_cap_size cap"
   apply (frule (1) well_formed_cap_object_is_real)
    apply (clarsimp simp: cap_has_object_def cap_type_def split: cdl_cap.splits)
   apply (clarsimp simp: well_formed_def split_def split:option.splits)
@@ -603,7 +601,7 @@ lemma slots_of_set [simp]:
 
 lemma well_formed_well_formed_tcb:
   "\<lbrakk>well_formed spec; cdl_objects spec obj_id = Some obj\<rbrakk>
-  \<Longrightarrow> well_formed_tcb spec obj_id obj"
+   \<Longrightarrow> well_formed_tcb spec obj_id obj"
   apply (clarsimp simp: well_formed_def)
   apply (erule_tac x=obj_id in allE)
   apply clarsimp
@@ -611,7 +609,7 @@ lemma well_formed_well_formed_tcb:
 
 lemma well_formed_well_formed_vspace:
   "\<lbrakk>well_formed spec; cdl_objects spec obj_id = Some obj\<rbrakk>
-  \<Longrightarrow> well_formed_vspace spec obj_id obj"
+   \<Longrightarrow> well_formed_vspace spec obj_id obj"
   apply (clarsimp simp: well_formed_def)
   apply (erule_tac x=obj_id in allE)
   apply clarsimp
@@ -619,7 +617,7 @@ lemma well_formed_well_formed_vspace:
 
 lemma well_formed_well_formed_irq_node:
   "\<lbrakk>well_formed spec; cdl_objects spec obj_id = Some obj\<rbrakk>
-  \<Longrightarrow> well_formed_irq_node spec obj_id obj"
+   \<Longrightarrow> well_formed_irq_node spec obj_id obj"
   apply (clarsimp simp: well_formed_def)
   apply (erule_tac x=obj_id in allE)
   apply clarsimp
@@ -640,7 +638,7 @@ lemma well_formed_inj_cdl_irq_node:
 lemma well_formed_vm_cap_has_asid:
   "\<lbrakk>well_formed spec; cdl_objects spec obj_id = Some obj;
     object_slots obj slot = Some cap\<rbrakk>
-  \<Longrightarrow> \<not>vm_cap_has_asid cap"
+   \<Longrightarrow> \<not>vm_cap_has_asid cap"
   apply (case_tac "cap = NullCap")
    apply (clarsimp simp: vm_cap_has_asid_def)
   apply (drule (3) well_formed_well_formed_cap)
@@ -655,27 +653,14 @@ lemma is_fake_vm_cap_cap_type:
   by (clarsimp simp: is_fake_vm_cap_def cap_type_def
               split: cdl_cap.splits)
 
-lemma well_formed_irq_node_in_irq_nodes:
-  "\<lbrakk>well_formed spec; cdl_objects spec obj_id = Some obj; is_irq_node obj\<rbrakk>
-  \<Longrightarrow> obj_id \<in> irq_nodes spec"
-  oops
-
-term real_object_at
-lemma well_formed_irq_node_cap_is_ntfn_cap:
-  "\<lbrakk>well_formed spec; cdl_objects spec obj_id = Some obj; is_irq_node obj;
-    object_slots obj slot = Some cap; cap \<noteq> NullCap\<rbrakk>
-  \<Longrightarrow> is_ntfn_cap cap"
-  apply (frule (3) well_formed_well_formed_cap_types_match)
-
-  apply (clarsimp simp: well_formed_cap_types_match_def)
-
-
-  oops
+lemma is_fake_vm_cap_cap_has_object[simp]:
+  "is_fake_vm_cap cap \<Longrightarrow> cap_has_object cap"
+  by (clarsimp simp: cap_has_object_def is_fake_vm_cap_def split: cdl_cap.splits)
 
 lemma well_formed_is_fake_vm_cap:
   "\<lbrakk>well_formed spec; cdl_objects spec obj_id = Some obj; is_cnode obj \<or> is_tcb obj \<or> is_irq_node obj;
     object_slots obj slot = Some cap\<rbrakk>
-  \<Longrightarrow> \<not>is_fake_vm_cap cap"
+   \<Longrightarrow> \<not>is_fake_vm_cap cap"
   apply (case_tac "is_irq_node obj")
    apply (frule (1) well_formed_well_formed_irq_node)
    apply (clarsimp simp: well_formed_irq_node_def object_at_def irq_nodes_def)
@@ -696,7 +681,7 @@ lemma vm_cap_has_asid_update_cap_object [simp]:
 
 lemma well_formed_object_size_bits_word_bits [simp]:
   "\<lbrakk>well_formed spec; cdl_objects spec obj_id = Some spec_obj\<rbrakk>
-  \<Longrightarrow> object_size_bits spec_obj < word_bits"
+   \<Longrightarrow> object_size_bits spec_obj < word_bits"
   apply (clarsimp simp: well_formed_def)
   apply (erule_tac x=obj_id in allE)
   apply clarsimp
@@ -705,7 +690,7 @@ lemma well_formed_object_size_bits_word_bits [simp]:
 lemma well_formed_is_untyped_cap:
   "\<lbrakk>well_formed spec; cnode_at obj_id spec;
     opt_cap (obj_id, slot) spec = Some cap\<rbrakk>
-  \<Longrightarrow> \<not> is_untyped_cap cap"
+   \<Longrightarrow> \<not> is_untyped_cap cap"
   apply (frule opt_cap_cdl_objects)
   apply (clarsimp simp: well_formed_def)
   apply (erule_tac x=obj_id in allE)
@@ -719,7 +704,7 @@ lemma well_formed_is_untyped_cap:
 lemma well_formed_cap_has_object:
   "\<lbrakk>well_formed spec; opt_cap (obj_id, slot) spec = Some spec_cap;
    spec_cap \<noteq> NullCap; \<not> is_untyped_cap spec_cap; \<not> is_irqhandler_cap spec_cap\<rbrakk>
-  \<Longrightarrow> cap_has_object spec_cap"
+   \<Longrightarrow> cap_has_object spec_cap"
   apply (clarsimp simp: opt_cap_def opt_object_def slots_of_def)
   apply (clarsimp simp: well_formed_def)
   apply (clarsimp split: option.splits)
@@ -736,7 +721,7 @@ lemma well_formed_cap_has_object:
 lemma well_formed_cap_object:
   "\<lbrakk>well_formed spec; opt_cap (obj_id, slot) spec = Some spec_cap;
     cap_has_object spec_cap\<rbrakk>
-  \<Longrightarrow> \<exists>obj. cdl_objects spec (cap_object spec_cap) = Some obj"
+   \<Longrightarrow> \<exists>obj. cdl_objects spec (cap_object spec_cap) = Some obj"
   apply (frule (1) well_formed_well_formed_cap', clarsimp)
   apply (frule (1) well_formed_cap_has_object)
     apply clarsimp
@@ -753,19 +738,19 @@ lemma well_formed_cap_object:
 lemma well_formed_cap_object_in_dom:
   "\<lbrakk>well_formed spec; opt_cap (obj_id, slot) spec = Some spec_cap;
     cap_has_object spec_cap\<rbrakk>
-  \<Longrightarrow> cap_object spec_cap \<in> dom (cdl_objects spec)"
+   \<Longrightarrow> cap_object spec_cap \<in> dom (cdl_objects spec)"
   by (drule (2) well_formed_cap_object, clarsimp)
 
 lemma well_formed_all_caps_cap_object:
   "\<lbrakk>well_formed spec; cap \<in> all_caps spec; cap_has_object cap\<rbrakk>
-  \<Longrightarrow>\<exists>obj. cdl_objects spec (cap_object cap) = Some obj"
+   \<Longrightarrow>\<exists>obj. cdl_objects spec (cap_object cap) = Some obj"
   apply (clarsimp simp: all_caps_def)
   apply (erule (2) well_formed_cap_object)
   done
 
 lemma well_formed_all_caps_cap_irq:
   "\<lbrakk>well_formed spec; cap \<in> all_caps spec; is_irqhandler_cap cap\<rbrakk>
-  \<Longrightarrow>\<exists>obj. cdl_objects spec (cdl_irq_node spec (cap_irq cap)) = Some obj"
+   \<Longrightarrow>\<exists>obj. cdl_objects spec (cdl_irq_node spec (cap_irq cap)) = Some obj"
   apply (clarsimp simp: all_caps_def)
   apply (frule (1) well_formed_well_formed_cap_types_match', simp)
   apply (clarsimp simp: well_formed_cap_types_match_def)
@@ -773,7 +758,7 @@ lemma well_formed_all_caps_cap_irq:
 
 lemma well_formed_update_cap_rights_idem:
   "\<lbrakk>well_formed_cap cap; rights = cap_rights cap\<rbrakk>
-  \<Longrightarrow> update_cap_rights rights cap = cap"
+   \<Longrightarrow> update_cap_rights rights cap = cap"
   by (auto simp: update_cap_rights_def cap_rights_def well_formed_cap_def
                validate_vm_rights_def vm_kernel_only_def vm_read_write_def
                vm_read_only_def split: cdl_cap.splits)
@@ -789,7 +774,7 @@ lemma default_ntfn_cap[simp]:
 
 lemma default_cap_well_formed_cap:
   "\<lbrakk>well_formed_cap cap; cap_type cap = Some type; cnode_cap_size cap = sz\<rbrakk>
-  \<Longrightarrow> well_formed_cap (default_cap type obj_ids sz dev)"
+   \<Longrightarrow> well_formed_cap (default_cap type obj_ids sz dev)"
   by (auto simp: well_formed_cap_def default_cap_def cap_type_def
                  word_gt_a_gt_0 vm_read_write_def cnode_cap_size_def
           split: cdl_cap.splits)
@@ -797,7 +782,7 @@ lemma default_cap_well_formed_cap:
 lemma default_cap_well_formed_cap2:
   "\<lbrakk>is_default_cap cap; cap_type cap = Some type; sz \<le> 32;
     \<not> is_untyped_cap cap; \<not> is_asidpool_cap cap\<rbrakk>
-  \<Longrightarrow> well_formed_cap (default_cap type obj_ids sz dev )"
+   \<Longrightarrow> well_formed_cap (default_cap type obj_ids sz dev )"
   apply (clarsimp simp: is_default_cap_def)
   apply (clarsimp simp: default_cap_def well_formed_cap_def
                         word_gt_a_gt_0 badge_bits_def guard_bits_def
@@ -809,7 +794,7 @@ lemma well_formed_well_formed_orig_cap:
   "\<lbrakk>well_formed spec;
     opt_cap (obj_id, slot) spec = Some cap; cap \<noteq> NullCap;
     original_cap_at (obj_id, slot) spec\<rbrakk>
-  \<Longrightarrow> well_formed_orig_cap cap"
+   \<Longrightarrow> well_formed_orig_cap cap"
   apply (frule opt_cap_dom_cdl_objects)
   apply (clarsimp simp: dom_def, rename_tac obj)
   apply (frule (1) object_slots_opt_cap, simp)
@@ -828,7 +813,7 @@ lemma well_formed_orig_ep_cap_is_default:
   "\<lbrakk>well_formed spec; original_cap_at (obj_id, slot) spec;
     opt_cap (obj_id, slot) spec = Some cap;
     ep_related_cap cap; cap \<noteq> NullCap\<rbrakk>
-  \<Longrightarrow> is_default_cap cap"
+   \<Longrightarrow> is_default_cap cap"
   apply (case_tac "\<exists>obj_id R. cap = ReplyCap obj_id R")
    apply (frule (1) well_formed_well_formed_cap', simp)
    apply (clarsimp simp: well_formed_cap_def)
@@ -847,7 +832,7 @@ lemma cap_rights_default_cap_eq:
 lemma well_formed_orig_caps:
   "\<lbrakk>well_formed spec; original_cap_at (obj_id, slot) spec;
     slots_of obj_id spec slot = Some cap; cap \<noteq> NullCap; cap_type cap = Some type\<rbrakk>
-  \<Longrightarrow> cap_rights (default_cap type obj_ids sz dev) = cap_rights cap"
+   \<Longrightarrow> cap_rights (default_cap type obj_ids sz dev) = cap_rights cap"
   apply (frule well_formed_well_formed_orig_cap, simp add: opt_cap_def, assumption+)
   apply (clarsimp simp: well_formed_orig_cap_def)
   apply (subst (asm) cap_rights_default_cap_eq, fast)
@@ -872,7 +857,7 @@ lemma well_formed_cdt:
 
 lemma well_formed_cap_to_real_object:
   "\<lbrakk>well_formed spec; real_object_at obj_id spec\<rbrakk>
-  \<Longrightarrow> \<exists>cnode_id slot cap.
+   \<Longrightarrow> \<exists>cnode_id slot cap.
        opt_cap (cnode_id, slot) spec = Some cap \<and>
        original_cap_at (cnode_id, slot) spec \<and>
        cnode_at cnode_id spec \<and>
@@ -885,7 +870,7 @@ lemma well_formed_cap_to_real_object:
 
 lemma well_formed_cap_to_irq_object:
   "\<lbrakk>well_formed spec; cdl_objects spec obj_id = Some obj; obj_id \<in> irq_nodes spec\<rbrakk>
-  \<Longrightarrow> \<exists>cnode_id slot cap.
+   \<Longrightarrow> \<exists>cnode_id slot cap.
        opt_cap (cnode_id, slot) spec = Some cap \<and>
        original_cap_at (cnode_id, slot) spec \<and>
        cnode_at cnode_id spec \<and>
@@ -898,7 +883,7 @@ lemma well_formed_cap_to_irq_object:
 lemma well_formed_cap_to_non_empty_pt:
   "\<lbrakk>well_formed spec; pt_at obj_id spec;
     object_at (\<lambda>obj. object_default_state obj \<noteq> obj) obj_id spec\<rbrakk>
-  \<Longrightarrow> \<exists>pd_id slot cap.
+   \<Longrightarrow> \<exists>pd_id slot cap.
        opt_cap (pd_id, slot) spec = Some cap \<and>
        pd_at pd_id spec \<and>
        cap_object cap = obj_id \<and>
@@ -915,21 +900,21 @@ lemma dom_object_slots_default_tcb:
 
 lemma well_formed_tcb_has_fault:
   "\<lbrakk>well_formed spec; cdl_objects spec obj_id = Some (Tcb tcb)\<rbrakk>
-  \<Longrightarrow> \<not> cdl_tcb_has_fault tcb"
+   \<Longrightarrow> \<not> cdl_tcb_has_fault tcb"
   apply (drule (1) well_formed_well_formed_tcb)
   apply (clarsimp simp: well_formed_tcb_def tcb_has_fault_def)
   done
 
 lemma well_formed_tcb_domain:
   "\<lbrakk>well_formed spec; cdl_objects spec obj_id = Some (Tcb tcb)\<rbrakk>
-  \<Longrightarrow> cdl_tcb_domain tcb = minBound"
+   \<Longrightarrow> cdl_tcb_domain tcb = minBound"
   apply (drule (1) well_formed_well_formed_tcb)
   apply (clarsimp simp: well_formed_tcb_def tcb_domain_def)
   done
 
 lemma well_formed_object_domain:
   "\<lbrakk>well_formed spec; cdl_objects spec obj_id = Some obj\<rbrakk>
-  \<Longrightarrow> object_domain obj = minBound"
+   \<Longrightarrow> object_domain obj = minBound"
   apply (case_tac "\<exists>tcb. obj = Tcb tcb")
    apply clarsimp
    apply (drule (1) well_formed_tcb_domain)
@@ -940,7 +925,7 @@ lemma well_formed_object_domain:
 
 lemma well_formed_tcb_object_slots:
   "\<lbrakk>well_formed spec; cdl_objects spec obj_id = Some tcb; is_tcb tcb\<rbrakk>
-  \<Longrightarrow> dom (object_slots tcb) = {0..tcb_boundntfn_slot}"
+   \<Longrightarrow> dom (object_slots tcb) = {0..tcb_boundntfn_slot}"
   apply (frule (1) well_formed_object_slots)
   apply (clarsimp simp: object_default_state_def2 is_tcb_def split: cdl_object.splits)
   apply (rule dom_object_slots_default_tcb)
@@ -949,7 +934,7 @@ lemma well_formed_tcb_object_slots:
 lemma well_formed_tcb_cspace_cap:
   "\<lbrakk>well_formed spec;
     tcb_at obj_id spec\<rbrakk>
-  \<Longrightarrow> \<exists>cspace_cap. opt_cap (obj_id, tcb_cspace_slot) spec = Some cspace_cap \<and>
+   \<Longrightarrow> \<exists>cspace_cap. opt_cap (obj_id, tcb_cspace_slot) spec = Some cspace_cap \<and>
                    is_cnode_cap cspace_cap \<and> cap_guard_size cspace_cap \<noteq> 0 \<and>
                    real_object_at (cap_object cspace_cap) spec"
   apply (clarsimp simp: object_at_def)
@@ -973,7 +958,7 @@ lemma well_formed_tcb_cspace_cap:
 
 lemma cap_data_cap_guard_size_0:
   "\<lbrakk>well_formed_cap cap; is_cnode_cap cap; cap_data cap = 0\<rbrakk>
-  \<Longrightarrow> cap_guard_size cap = 0"
+   \<Longrightarrow> cap_guard_size cap = 0"
   apply (clarsimp simp: cap_type_def cap_data_def guard_as_rawdata_def
                         well_formed_cap_def
                  split: cdl_cap.splits)
@@ -993,7 +978,7 @@ lemma well_formed_tcb_cspace_cap_cap_data:
   "\<lbrakk>well_formed spec; tcb_at obj_id spec;
     cdl_objects spec obj_id = Some (Tcb tcb);
     opt_cap (obj_id, tcb_cspace_slot) spec = Some spec_cspace_cap\<rbrakk>
-  \<Longrightarrow> cap_data spec_cspace_cap \<noteq> 0"
+   \<Longrightarrow> cap_data spec_cspace_cap \<noteq> 0"
   apply (frule (1) well_formed_tcb_cspace_cap, clarsimp)
   apply (frule (1) well_formed_well_formed_cap', clarsimp)
   apply (drule (2) cap_data_cap_guard_size_0, simp)
@@ -1001,7 +986,7 @@ lemma well_formed_tcb_cspace_cap_cap_data:
 
 lemma well_formed_tcb_opt_cap:
   "\<lbrakk>well_formed spec; tcb_at obj_id spec; slot \<in> {0..tcb_boundntfn_slot}\<rbrakk>
-  \<Longrightarrow> \<exists>cap. opt_cap (obj_id, slot) spec = Some cap"
+   \<Longrightarrow> \<exists>cap. opt_cap (obj_id, slot) spec = Some cap"
   apply (clarsimp simp: object_at_def)
   apply (drule (1) well_formed_object_slots)
   apply (fastforce simp: object_default_state_def2 is_tcb_def
@@ -1014,7 +999,7 @@ lemma well_formed_tcb_opt_cap:
 lemma well_formed_tcb_vspace_cap:
   "\<lbrakk>well_formed spec;
     tcb_at obj_id spec\<rbrakk>
-  \<Longrightarrow> \<exists>vspace_cap.
+   \<Longrightarrow> \<exists>vspace_cap.
     opt_cap (obj_id, tcb_vspace_slot) spec = Some vspace_cap \<and> is_pd_cap vspace_cap"
   apply (frule (1) well_formed_tcb_opt_cap [where slot=tcb_vspace_slot], simp add: tcb_slot_defs)
   apply (clarsimp simp: object_at_def)
@@ -1025,7 +1010,7 @@ lemma well_formed_tcb_vspace_cap:
 lemma well_formed_tcb_ipcbuffer_cap:
   "\<lbrakk>well_formed spec;
     tcb_at obj_id spec\<rbrakk>
-  \<Longrightarrow> \<exists>tcb_ipcbuffer_cap.
+   \<Longrightarrow> \<exists>tcb_ipcbuffer_cap.
     opt_cap (obj_id, tcb_ipcbuffer_slot) spec = Some tcb_ipcbuffer_cap \<and>
     is_default_cap tcb_ipcbuffer_cap \<and> is_frame_cap tcb_ipcbuffer_cap"
   apply (frule (1) well_formed_tcb_opt_cap [where slot=tcb_ipcbuffer_slot], simp add: tcb_slot_defs)
@@ -1036,7 +1021,7 @@ lemma well_formed_tcb_ipcbuffer_cap:
 
 lemma well_formed_tcb_caller_cap:
   "\<lbrakk>well_formed spec; tcb_at obj_id spec\<rbrakk>
-  \<Longrightarrow> opt_cap (obj_id, tcb_caller_slot) spec = Some NullCap"
+   \<Longrightarrow> opt_cap (obj_id, tcb_caller_slot) spec = Some NullCap"
   apply (frule (1) well_formed_tcb_opt_cap [where slot=tcb_caller_slot], simp add: tcb_slot_defs)
   apply (clarsimp simp: object_at_def)
   apply (frule (1) well_formed_well_formed_tcb)
@@ -1045,7 +1030,7 @@ lemma well_formed_tcb_caller_cap:
 
 lemma well_formed_tcb_replycap_cap:
   "\<lbrakk>well_formed spec; tcb_at obj_id spec\<rbrakk>
-  \<Longrightarrow> opt_cap (obj_id, tcb_replycap_slot) spec = Some NullCap \<or>
+   \<Longrightarrow> opt_cap (obj_id, tcb_replycap_slot) spec = Some NullCap \<or>
       opt_cap (obj_id, tcb_replycap_slot) spec = Some (MasterReplyCap obj_id)"
   apply (frule (1) well_formed_tcb_opt_cap [where slot=tcb_replycap_slot], simp add: tcb_slot_defs)
   apply (clarsimp simp: object_at_def)
@@ -1056,7 +1041,7 @@ lemma well_formed_tcb_replycap_cap:
 
 lemma well_formed_tcb_pending_op_cap:
   "\<lbrakk>well_formed spec; tcb_at obj_id spec\<rbrakk>
-  \<Longrightarrow> opt_cap (obj_id, tcb_pending_op_slot) spec = Some NullCap \<or>
+   \<Longrightarrow> opt_cap (obj_id, tcb_pending_op_slot) spec = Some NullCap \<or>
       opt_cap (obj_id, tcb_pending_op_slot) spec = Some RestartCap"
   apply (frule (1) well_formed_tcb_opt_cap [where slot=tcb_pending_op_slot], simp add: tcb_slot_defs)
   apply (clarsimp simp: object_at_def)
@@ -1066,7 +1051,7 @@ lemma well_formed_tcb_pending_op_cap:
 
 lemma well_formed_tcb_pending_op_replycap:
   "\<lbrakk>well_formed spec; tcb_at obj_id spec\<rbrakk>
-  \<Longrightarrow> (opt_cap (obj_id, tcb_replycap_slot) spec = Some (MasterReplyCap obj_id))
+   \<Longrightarrow> (opt_cap (obj_id, tcb_replycap_slot) spec = Some (MasterReplyCap obj_id))
     = (opt_cap (obj_id, tcb_pending_op_slot) spec = Some RestartCap)"
   apply (clarsimp simp: object_at_def)
   apply (drule (1) well_formed_well_formed_tcb)
@@ -1075,7 +1060,7 @@ lemma well_formed_tcb_pending_op_replycap:
 
 lemma well_formed_tcb_boundntfn_cap:
   "\<lbrakk>well_formed spec; tcb_at obj_id spec\<rbrakk>
-  \<Longrightarrow> opt_cap (obj_id, tcb_boundntfn_slot) spec = Some NullCap"
+   \<Longrightarrow> opt_cap (obj_id, tcb_boundntfn_slot) spec = Some NullCap"
   apply (frule (1) well_formed_tcb_opt_cap [where slot=tcb_boundntfn_slot], simp add: tcb_slot_defs)
   apply (elim exE)
   apply (clarsimp simp: object_at_def)
@@ -1087,7 +1072,7 @@ lemma well_formed_orig_caps_unique:
     cnode_at obj_id spec; cnode_at obj_id' spec; cap_has_object cap; cap_has_object cap';
     opt_cap (obj_id, slot) spec = Some cap; opt_cap (obj_id', slot') spec = Some cap';
     cap_object cap = cap_object cap'\<rbrakk>
-  \<Longrightarrow> obj_id = obj_id' \<and> slot = slot'"
+   \<Longrightarrow> obj_id = obj_id' \<and> slot = slot'"
   by (clarsimp simp: well_formed_def well_formed_orig_caps_unique_def)
 
 lemma well_formed_orig_caps_unique':
@@ -1096,19 +1081,19 @@ lemma well_formed_orig_caps_unique':
     opt_cap (obj_id, slot) spec = Some cap; opt_cap (obj_id', slot') spec = Some cap';
     cap_has_object cap; cap_has_object cap';
     cap_object cap = cap_object cap'\<rbrakk>
-  \<Longrightarrow> obj_id = obj_id' \<and> slot = slot'"
+   \<Longrightarrow> obj_id = obj_id' \<and> slot = slot'"
   by (clarsimp simp: well_formed_def well_formed_orig_caps_unique_def real_cap_ref_def)
 
 lemma well_formed_irqhandler_caps_unique:
   "\<lbrakk>well_formed s; is_irqhandler_cap cap; is_irqhandler_cap cap';
     opt_cap (obj_id, slot) s = Some cap; opt_cap (obj_id', slot') s = Some cap';
     cap_irq cap = cap_irq cap'\<rbrakk>
-  \<Longrightarrow> obj_id = obj_id' \<and> slot = slot'"
+   \<Longrightarrow> obj_id = obj_id' \<and> slot = slot'"
   by (clarsimp simp: well_formed_def well_formed_irqhandler_caps_unique_def)
 
 lemma object_cap_ref_cap_irq:
   "\<lbrakk>object_cap_ref (obj_id, slot) spec; opt_cap (obj_id, slot) spec = Some cap\<rbrakk>
-  \<Longrightarrow> cap_irq cap = undefined"
+   \<Longrightarrow> cap_irq cap = undefined"
   by (auto simp: object_cap_ref_def cap_has_object_def cap_irq_def
           split: cdl_cap.splits)
 
@@ -1122,7 +1107,7 @@ lemma well_formed_orig_caps_unique_object_cap:
     opt_cap (obj_id, slot) spec = Some cap; opt_cap (obj_id', slot') spec = Some cap';
     cap_has_object cap; cap_has_object cap';
     cap_object cap = cap_object cap'\<rbrakk>
-  \<Longrightarrow> obj_id = obj_id' \<and> slot = slot'"
+   \<Longrightarrow> obj_id = obj_id' \<and> slot = slot'"
   apply (frule object_cap_ref_real_cap_ref, drule (1) object_cap_ref_cap_irq)+
   apply (erule (8) well_formed_orig_caps_unique', simp)
   done
@@ -1130,7 +1115,7 @@ lemma well_formed_orig_caps_unique_object_cap:
 lemma well_formed_child_cap_not_copyable:
   "\<lbrakk>well_formed spec; \<not> original_cap_at (obj_id, slot) spec;
     opt_cap (obj_id, slot) spec = Some cap; cap \<noteq> NullCap\<rbrakk>
-  \<Longrightarrow> is_copyable_cap cap"
+   \<Longrightarrow> is_copyable_cap cap"
   apply (clarsimp simp: well_formed_def)
   apply (erule_tac x=obj_id in allE)
   apply (clarsimp simp: opt_cap_def opt_object_def slots_of_def)
@@ -1142,13 +1127,13 @@ lemma well_formed_child_cap_not_copyable:
 lemma well_formed_child_cap_not_copyable':
   "\<lbrakk>well_formed spec;
     opt_cap (obj_id, slot) spec = Some cap; cap \<noteq> NullCap\<rbrakk>
-  \<Longrightarrow> \<not>original_cap_at (obj_id, slot) spec \<longrightarrow> is_copyable_cap cap"
+   \<Longrightarrow> \<not>original_cap_at (obj_id, slot) spec \<longrightarrow> is_copyable_cap cap"
   by (rule impI, erule (3) well_formed_child_cap_not_copyable)
 
 lemma well_formed_pd:
   "\<lbrakk>well_formed spec; opt_cap (obj_id, slot) spec = Some cap;
     pd_at obj_id spec; cap \<noteq> NullCap\<rbrakk>
-  \<Longrightarrow> is_frame_cap cap \<or> is_fake_pt_cap cap"
+   \<Longrightarrow> is_frame_cap cap \<or> is_fake_pt_cap cap"
   apply (clarsimp simp: object_at_def)
   apply (frule (1) well_formed_well_formed_vspace)
   apply (clarsimp simp: well_formed_vspace_def)
@@ -1160,7 +1145,7 @@ lemma well_formed_pd:
 lemma well_formed_pt:
   "\<lbrakk>well_formed spec; opt_cap (obj_id, slot) spec = Some cap;
     pt_at obj_id spec; cap \<noteq> NullCap\<rbrakk>
-  \<Longrightarrow> is_frame_cap cap"
+   \<Longrightarrow> is_frame_cap cap"
   apply (clarsimp simp: object_at_def)
   apply (frule (1) well_formed_well_formed_vspace)
   apply (clarsimp simp: well_formed_vspace_def)
@@ -1175,6 +1160,26 @@ lemma well_formed_pt_cap_is_fake_pt_cap:
    \<Longrightarrow> is_fake_pt_cap cap"
   by (frule (2) well_formed_pd, clarsimp+)
 
+lemma wf_cap_pt_cap[simp]: "well_formed_cap (PageTableCap pt_id ty addr) \<longleftrightarrow> addr = None"
+  by (clarsimp simp: well_formed_cap_def)
+
+lemma wf_frame_cap_frame_size_bits:
+  "\<lbrakk>well_formed spec;
+    opt_cap (pt_ptr, slot) spec = Some (FrameCap dev frame_ptr rights n Fake None);
+    cdl_objects spec frame_ptr = Some (Frame frame)\<rbrakk>
+   \<Longrightarrow> cdl_frame_size_bits frame = n"
+  apply (clarsimp simp: opt_cap_def slots_of_def opt_object_def split: option.splits)
+  apply (frule (2) well_formed_well_formed_cap_types_match, fastforce)
+  apply (fastforce simp: well_formed_cap_types_match_def cap_object_def object_type_def)
+  done
+
+lemma wf_pd_cap_has_object:
+  "\<lbrakk>well_formed spec;
+    pd_at spec_pd_ptr spec;
+    opt_cap (spec_pd_ptr, slot) spec = Some cap;
+    cap \<noteq> NullCap\<rbrakk> \<Longrightarrow> cap_has_object cap"
+  by (fastforce simp: cap_has_object_def cap_type_def is_fake_pt_cap_def
+                dest: well_formed_pd split: cdl_cap.splits)
 
 
 (****************************************
@@ -1237,7 +1242,7 @@ lemma well_formed_irq_nodes_cdl_irq_node:
 
 lemma well_formed_cdl_irq_node_irq_nodes:
   "\<lbrakk>well_formed spec; cdl_objects spec (cdl_irq_node spec irq) = Some irq_node\<rbrakk>
-  \<Longrightarrow> cdl_irq_node spec irq \<in> irq_nodes spec"
+   \<Longrightarrow> cdl_irq_node spec irq \<in> irq_nodes spec"
   apply (drule well_formed_well_formed_irq_table)
   apply (clarsimp simp: well_formed_irq_table_def)
   apply (fastforce simp: object_at_def)
@@ -1245,14 +1250,14 @@ lemma well_formed_cdl_irq_node_irq_nodes:
 
 lemma well_formed_irq_is_irq_node:
   "\<lbrakk>well_formed spec; cdl_objects spec (cdl_irq_node spec irq) = Some irq_node\<rbrakk>
-  \<Longrightarrow> is_irq_node irq_node"
+   \<Longrightarrow> is_irq_node irq_node"
   apply (frule (1) well_formed_cdl_irq_node_irq_nodes)
   apply (clarsimp simp: irq_nodes_def object_at_def)
   done
 
 lemma well_formed_object_slots_irq_node:
   "\<lbrakk>well_formed spec; cdl_objects spec (cdl_irq_node spec irq) = Some irq_node\<rbrakk>
-  \<Longrightarrow> dom (object_slots irq_node) = {0}"
+   \<Longrightarrow> dom (object_slots irq_node) = {0}"
   apply (frule (1) well_formed_cdl_irq_node_irq_nodes)
   apply (frule (1) well_formed_well_formed_irq_node)
   apply (clarsimp simp: well_formed_irq_node_def)
@@ -1262,7 +1267,7 @@ lemma well_formed_irq_ntfn_cap:
   "\<lbrakk>well_formed spec;
     irq \<in> bound_irqs spec;
     opt_cap (cdl_irq_node spec irq, 0) spec = Some ntfn_cap\<rbrakk>
-  \<Longrightarrow> ntfn_cap = NotificationCap (cap_object ntfn_cap) 0 {AllowRead, AllowWrite}"
+   \<Longrightarrow> ntfn_cap = NotificationCap (cap_object ntfn_cap) 0 {AllowRead, AllowWrite}"
   apply (frule opt_cap_cdl_objects, clarsimp)
   apply (frule (1) well_formed_object_slots_irq_node [where irq=irq])
   apply (frule (1) well_formed_well_formed_irq_node)
@@ -1284,7 +1289,7 @@ lemma well_formed_bound_irqs_are_used_irqs:
 
 lemma well_formed_slots_of_used_irq_node:
   "\<lbrakk>well_formed spec; irq \<in> used_irqs spec\<rbrakk>
-  \<Longrightarrow> dom (slots_of (cdl_irq_node spec irq) spec) = {0}"
+   \<Longrightarrow> dom (slots_of (cdl_irq_node spec irq) spec) = {0}"
   apply (clarsimp simp: used_irqs_def slots_of_def opt_object_def split: option.splits)
   apply (frule (2) well_formed_all_caps_cap_irq, clarsimp)
   apply (erule (1) well_formed_object_slots_irq_node)
@@ -1292,14 +1297,14 @@ lemma well_formed_slots_of_used_irq_node:
 
 lemma well_formed_slot_0_of_used_irq_node:
   "\<lbrakk>well_formed spec; irq \<in> used_irqs spec\<rbrakk>
-  \<Longrightarrow> \<exists>ntfn_cap. slots_of (cdl_irq_node spec irq) spec 0 = Some ntfn_cap"
+   \<Longrightarrow> \<exists>ntfn_cap. slots_of (cdl_irq_node spec irq) spec 0 = Some ntfn_cap"
   apply (frule (1) well_formed_slots_of_used_irq_node)
   apply (clarsimp simp: dom_eq_singleton_conv)
   done
 
 lemma well_formed_object_slots_default_irq_node:
   "\<lbrakk>well_formed spec; cdl_objects spec (cdl_irq_node spec irq) = Some irq_node\<rbrakk>
-  \<Longrightarrow> dom (object_slots (object_default_state irq_node)) = {0}"
+   \<Longrightarrow> dom (object_slots (object_default_state irq_node)) = {0}"
   by (metis well_formed_object_slots well_formed_object_slots_irq_node)
 
 lemma object_slots_empty_cnode:
@@ -1315,7 +1320,7 @@ lemma dom_empty_cap_map_singleton:
 
 lemma well_formed_size_irq_node:
   "\<lbrakk>well_formed spec; cdl_objects spec (cdl_irq_node spec irq) = Some irq_node\<rbrakk>
-  \<Longrightarrow> object_size_bits irq_node = 0"
+   \<Longrightarrow> object_size_bits irq_node = 0"
   apply (frule (1) well_formed_irq_is_irq_node)
   apply (frule (1) well_formed_object_slots)
   apply (drule (1) well_formed_object_slots_default_irq_node)
@@ -1326,14 +1331,14 @@ lemma well_formed_size_irq_node:
 
 lemma well_formed_used_irqs_have_irq_node:
   "\<lbrakk>well_formed spec; irq \<in> used_irqs spec\<rbrakk>
-  \<Longrightarrow> \<exists>irq_node. cdl_objects spec (cdl_irq_node spec irq) = Some irq_node"
+   \<Longrightarrow> \<exists>irq_node. cdl_objects spec (cdl_irq_node spec irq) = Some irq_node"
   apply (clarsimp simp: used_irqs_def)
   apply (erule (2) well_formed_all_caps_cap_irq)
   done
 
 lemma well_formed_bound_irqs_have_irq_node:
   "\<lbrakk>well_formed spec; irq \<in> bound_irqs spec\<rbrakk>
-  \<Longrightarrow> \<exists>irq_node. cdl_objects spec (cdl_irq_node spec irq) = Some irq_node"
+   \<Longrightarrow> \<exists>irq_node. cdl_objects spec (cdl_irq_node spec irq) = Some irq_node"
   apply (frule well_formed_well_formed_irqhandler_caps)
   apply (clarsimp simp: well_formed_irqhandler_caps_def used_irqs_def bound_irqs_def all_caps_def)
   done
@@ -1341,7 +1346,7 @@ lemma well_formed_bound_irqs_have_irq_node:
 lemma well_formed_irq_node_is_bound:
   "\<lbrakk>well_formed spec; cdl_objects spec (cdl_irq_node spec irq) = Some irq_node;
     object_slots irq_node 0 \<noteq> Some NullCap\<rbrakk>
-  \<Longrightarrow> irq \<in> bound_irqs spec"
+   \<Longrightarrow> irq \<in> bound_irqs spec"
   apply (frule well_formed_well_formed_irqhandler_caps)
   apply (frule (1) well_formed_object_slots_default_irq_node)
   apply (frule (1) well_formed_object_slots)
@@ -1376,7 +1381,7 @@ lemma well_formed_cap_object_cdl_irq_node:
 (* There are no untyped objects (as there are no untyped caps). *)
 lemma well_formed_object_untyped:
  "\<lbrakk>well_formed spec; cdl_objects spec obj_id = Some object\<rbrakk>
-  \<Longrightarrow> object_type object \<noteq> UntypedType"
+   \<Longrightarrow> object_type object \<noteq> UntypedType"
   apply (case_tac "real_object_at obj_id spec")
    apply (frule (1) well_formed_cap_to_real_object)
    apply clarsimp
@@ -1411,7 +1416,7 @@ lemma well_formed_no_asidpools:
 
 lemma well_formed_fake_pt_cap_in_pd:
   "\<lbrakk>well_formed spec; slots_of obj_id spec slot = Some cap; is_fake_pt_cap cap\<rbrakk>
-  \<Longrightarrow> pd_at obj_id spec"
+   \<Longrightarrow> pd_at obj_id spec"
   apply (clarsimp simp: slots_of_def opt_object_def split: option.splits)
   apply (rename_tac obj)
   apply (frule well_formed_asidpool_at [where obj_id=obj_id])
@@ -1426,6 +1431,18 @@ lemma well_formed_fake_pt_cap_in_pd:
   apply (erule allE [where x=slot])
   apply (erule allE [where x=cap])
   apply (clarsimp simp: is_fake_pt_cap_is_pt_cap object_slots_def)
+  done
+
+lemma well_formed_pt_cap_pt_at:
+  "\<lbrakk>well_formed spec; opt_cap cap_ref spec = Some cap; is_fake_pt_cap cap\<rbrakk>
+   \<Longrightarrow> pt_at (cap_object cap) spec"
+  apply (case_tac cap_ref, clarsimp)
+  apply (frule (1) well_formed_cap_object)
+   apply (fastforce intro: is_fake_pt_cap_cap_has_object)
+  apply clarsimp
+  apply (frule (2) well_formed_types_match)
+   apply (fastforce intro: is_fake_pt_cap_cap_has_object)
+  apply (clarsimp simp: is_fake_pt_cap_is_pt_cap object_at_def object_type_is_object)
   done
 
 lemma cap_has_object_cap_irq [simp]:
@@ -1573,7 +1590,7 @@ lemma well_formed_objects_only_real_or_irq:
 
 lemma well_formed_objects_card:
   "\<lbrakk>well_formed spec \<rbrakk>
-  \<Longrightarrow> card (used_irqs spec) + card {x. real_object_at x spec} = card (dom (cdl_objects spec))"
+   \<Longrightarrow> card (used_irqs spec) + card {x. real_object_at x spec} = card (dom (cdl_objects spec))"
   apply (frule well_formed_inj_cdl_irq_node)
   apply (frule well_formed_objects_real_or_irq)
   apply (frule well_formed_objects_only_real_or_irq)
@@ -1672,6 +1689,153 @@ lemma update_cap_data:
    apply (subst cap_rights_default_cap_eq, fast)
   apply simp
   done
+
+lemma well_formed_frame_in_pt:
+  "\<lbrakk>well_formed spec;
+    opt_cap (pt, pt_slot) spec = Some frame_cap;
+    frame_cap \<noteq> NullCap;
+    pt_at pt spec\<rbrakk>
+   \<Longrightarrow> \<exists>sz. cap_type frame_cap = Some (FrameType sz) \<and>
+           (sz = 12 \<or> sz = 16) \<and>
+           is_fake_vm_cap frame_cap"
+  apply (clarsimp simp: well_formed_def object_at_def)
+  apply (drule_tac x = pt in spec)
+  apply (clarsimp simp: well_formed_vspace_def opt_cap_def slots_of_def opt_object_def
+                 split: option.split_asm)
+  done
+
+lemma well_formed_frame_in_pd:
+  "\<lbrakk>well_formed spec;
+    opt_cap (pd, pt_slot) spec = Some frame_cap;
+    pd_at pd spec;
+    is_frame_cap frame_cap\<rbrakk>
+   \<Longrightarrow> (\<exists>sz. cap_type frame_cap = Some (FrameType sz) \<and> (sz = 20 \<or> sz = 24)) \<and>
+      is_fake_vm_cap frame_cap \<and>
+      \<not> is_device_cap frame_cap"
+  apply (clarsimp simp: well_formed_def object_at_def)
+  apply (drule_tac x = pd in spec)
+  apply (clarsimp simp: well_formed_vspace_def opt_cap_def slots_of_def opt_object_def
+                 split: option.split_asm)
+  apply (drule_tac x = pt_slot in spec)
+  apply (drule_tac x = frame_cap in spec)
+  apply (clarsimp simp: is_fake_pt_cap_def cap_type_def
+                 split: cdl_cap.splits)
+  apply (clarsimp simp: cap_at_def opt_cap_def slots_of_def opt_object_def
+              simp del: split_paired_All)
+  apply (drule_tac x = pd in spec)
+  apply (drule_tac x = pt_slot in spec)
+  apply fastforce
+  done
+
+lemma well_formed_no_dev: "well_formed spec \<Longrightarrow> \<forall>slot. \<not> cap_at is_device_cap slot spec"
+  by (clarsimp simp: well_formed_def)
+
+lemma well_formed_frame_cap[simp]:
+  "well_formed_cap (FrameCap x y rights a b R) \<longleftrightarrow>
+     R = None \<and> (rights = vm_read_write \<or> rights = vm_read_only)"
+  apply (clarsimp simp: well_formed_cap_def split: cdl_frame_cap_type.splits)
+  apply (rule iffI; clarsimp?)
+  done
+
+lemma wf_cap_in_pt_is_frame:
+  "well_formed spec \<Longrightarrow>
+   page_cap \<noteq> NullCap \<Longrightarrow>
+   pt_at pt_id spec \<Longrightarrow>
+   opt_cap (pt_id, slot) spec = Some page_cap \<Longrightarrow>
+   page_cap = fake_frame_cap False (cap_object page_cap)
+                                   (validate_vm_rights (cap_rights page_cap))
+                                   (cap_size_bits page_cap) \<and>
+  (cap_size_bits page_cap = 12 \<or> cap_size_bits page_cap = 16)"
+  apply (frule well_formed_frame_in_pt, fastforce+)
+  apply (clarsimp simp: cap_type_def cap_rights_def cap_size_bits_def split: cdl_cap.splits)
+  apply (frule well_formed_well_formed_cap[where obj_id=pt_id])
+     apply (fastforce intro: object_slots_opt_capI)+
+  apply clarsimp
+  apply (drule well_formed_no_dev, clarsimp simp: cap_at_def)
+  apply (fastforce simp: fake_vm_cap_simp)
+  done
+
+lemma wf_frame_cap_in_pd:
+  "well_formed spec \<Longrightarrow>
+   page_cap \<noteq> NullCap \<Longrightarrow>
+   pd_at pd_id spec \<Longrightarrow>
+   opt_cap (pd_id, slot) spec = Some page_cap \<Longrightarrow>
+   frame_at (cap_object page_cap) spec \<Longrightarrow>
+   page_cap = fake_frame_cap False (cap_object page_cap)
+                                   (validate_vm_rights (cap_rights page_cap))
+                                   (cap_size_bits page_cap) \<and>
+   (cap_size_bits page_cap = 20 \<or> cap_size_bits page_cap = 24)"
+  apply (frule well_formed_frame_in_pd, fastforce+)
+   apply (frule well_formed_types_match, fastforce+)
+    using object_type_is_object(9) object_type_object_at(9) wf_pd_cap_has_object apply blast
+   apply (frule object_at_object_type(10)[rotated], rule classical, fastforce)
+   apply (fastforce simp: cap_type_def split: cdl_cap.splits)
+  apply (clarsimp simp: cap_type_def cap_rights_def cap_size_bits_def split: cdl_cap.splits)
+  apply (frule well_formed_well_formed_cap[where obj_id=pd_id])
+     apply fastforce
+    apply (fastforce intro: object_slots_opt_capI)
+   apply (fastforce simp: fake_vm_cap_simp)+
+  done
+
+lemma wf_pt_in_pd_fake_and_none:
+  "well_formed spec \<Longrightarrow>
+   page_cap \<noteq> NullCap \<Longrightarrow>
+   pd_at pd_id spec \<Longrightarrow>
+   opt_cap (pd_id, slot) spec = Some page_cap \<Longrightarrow>
+   pt_at (cap_object page_cap) spec \<Longrightarrow>
+   page_cap = PageTableCap (cap_object page_cap) Fake None"
+  apply (clarsimp simp: object_at_def)
+  apply (frule well_formed_types_match[where obj_id=pd_id and slot=slot])
+     apply fastforce+
+     using object_at_def wf_pd_cap_has_object
+   apply blast
+  apply (clarsimp simp: object_type_is_object)
+  apply (frule well_formed_pt_cap_is_fake_pt_cap[where obj_id=pd_id and slot=slot])
+     apply fastforce
+    apply (clarsimp simp: object_at_def)
+    apply (clarsimp simp: object_type_is_object)
+   apply (frule (1) well_formed_well_formed_cap[where obj_id=pd_id and slot=slot])
+     apply (clarsimp simp: opt_cap_def slots_of_def opt_object_def split: option.splits)
+     apply fastforce+
+  apply (clarsimp simp: cap_type_def is_fake_pt_cap_pt_cap split: cdl_cap.splits)
+  using well_formed_well_formed_cap' wf_cap_pt_cap by blast
+
+lemma well_formed_pd_slots_have_objects:
+  "\<lbrakk>well_formed spec; pd_at pd_id spec; slot \<in> dom (slots_of pd_id spec);
+    slots_of pd_id spec slot = Some cap; cap \<noteq> NullCap\<rbrakk>
+   \<Longrightarrow> cap_has_object cap"
+  apply (drule (1) wf_pd_cap_has_object[where cap=cap and slot=slot])
+    apply (clarsimp simp: opt_cap_def)+
+  done
+
+lemma well_formed_pd_slot_limited:
+  "\<lbrakk>well_formed spec; pd_at obj_id spec; slots_of obj_id spec slot = Some cap\<rbrakk>
+   \<Longrightarrow> slot < 4096"
+  apply (clarsimp simp:well_formed_def object_at_def)
+  apply (drule_tac x = obj_id in spec)
+  apply (clarsimp simp: is_pd_def object_type_simps object_default_state_def slots_of_def,
+              simp add: default_object_def object_type_simps opt_object_def object_slots_def empty_cap_map_def
+                 split: cdl_object.split_asm option.split_asm)
+  apply fastforce
+  done
+
+lemma well_formed_pd_frame_or_pt:
+  "well_formed spec \<Longrightarrow>
+   pd_at pd_ptr spec \<Longrightarrow>
+   opt_cap (pd_ptr,slot) spec = Some slot_cap \<Longrightarrow>
+   cap_object slot_cap = ptr \<Longrightarrow>
+   slot_cap \<noteq> NullCap \<Longrightarrow>
+   frame_at ptr spec \<noteq> pt_at ptr spec"
+  apply (frule (3) well_formed_pd[where obj_id=pd_ptr and slot=slot])
+  apply clarsimp
+  apply (frule (3) wf_pd_cap_has_object)
+  apply (frule (2) well_formed_cap_object)
+  apply clarsimp
+  apply (safe; (fastforce simp: object_at_def dest: not_frame_and_pt)?)
+   apply (frule well_formed_types_match[where obj_id=pd_ptr and slot=slot], fastforce+)
+   apply (fastforce simp: object_type_is_object(10) intro: object_at_cdl_objects)
+  apply (frule well_formed_types_match[where obj_id=pd_ptr and slot=slot], fastforce+)
+  using is_fake_pt_cap_is_pt_cap object_type_is_object(8) by (fastforce intro: object_at_cdl_objects)
 
 end
 
