sys-init/Mapped_Separating_Conjunction.thy
@@ -1,0 +1,216 @@
+(*
+ * Copyright 2019, Data61
+ *
+ * This software may be distributed and modified according to the terms of
+ * the GNU General Public License version 2. Note that NO WARRANTY is provided.
+ * See "LICENSE_GPLv2.txt" for details.
+ *
+ * @TAG(DATA61_GPL)
+ *)
+
+(* Utility lemmas related to the mapping of separating conjunctions over sets and lists *)
+
+theory Mapped_Separating_Conjunction
+imports
+  Sep_Algebra.Sep_Algebra_L4v
+  "HOL-Library.Multiset"
+begin
+
+lemmas sep_map_set_conj_set_cong = arg_cong[where f="sep_map_set_conj P" for P]
+
+lemma sep_map_set_conj_set_elim:
+  "sep_map_set_conj P xs s \<Longrightarrow> \<lbrakk> \<And>x s. x \<in> xs \<Longrightarrow> P x s = Q x s\<rbrakk> \<Longrightarrow>  sep_map_set_conj Q xs s"
+  apply (induct xs arbitrary: s rule: infinite_finite_induct)
+    apply fastforce
+   apply fastforce
+  apply clarsimp
+  apply (erule sep_conj_impl; blast)
+  done
+
+lemma split_filter_set: "xs = {x \<in> xs. P x} \<union> {x \<in> xs. \<not>P x}"
+  by blast
+
+lemma set_minus_not_filter[simp]: "{x \<in> xs. P x} - {x \<in> xs. \<not>P x} = {x \<in> xs. P x}"
+  by blast
+
+lemma set_minus_not_filter'[simp]: "{x \<in> xs. \<not>P x} - {x \<in> xs. P x} = {x \<in> xs. \<not>P x}"
+  by blast
+
+lemma set_inter_not_filter[simp]: "{x \<in> xs. P x} \<inter> {x \<in> xs. \<not>P x} = {}"
+  by blast
+
+declare sep_list_conj_map_add[simp]
+
+lemma sep_map_list_conj_decomp[simp]:
+  "sep_map_list_conj (\<lambda>(x, y). P x y \<and>* Q x y) xs =
+     (sep_map_list_conj (\<lambda>(x, y). P x y) xs \<and>* sep_map_list_conj (\<lambda>(x , y). Q x y) xs)"
+  apply (intro ext iffI)
+   apply (induct xs; clarsimp)
+   apply sep_cancel+
+   apply fastforce
+  apply (induct xs; clarsimp)
+  apply sep_cancel+
+  apply fastforce
+  done
+
+lemma image_insertD: "insert (P x) (P ` S) = Q ` S' \<Longrightarrow> \<exists>s\<in>S'. Q s = P x "
+  by (metis imageE insertI1)
+
+lemma sep_map_set_inj_eqI:
+  "inj_on P xs \<Longrightarrow> inj_on Q ys \<Longrightarrow> P ` xs = Q ` ys \<Longrightarrow>
+   sep_map_set_conj P xs = sep_map_set_conj Q ys"
+  apply (induct xs arbitrary: ys rule: infinite_finite_induct)
+    apply clarsimp
+    defer
+    apply clarsimp+
+   apply (frule image_insertD)
+   apply clarsimp
+   apply atomize
+   apply (erule_tac x="ys - {s}" in allE)
+   apply (drule mp)
+    apply (simp add: inj_on_diff)
+   apply (drule mp)
+    apply (metis (no_types, hide_lams) image_insert inj_on_insert insert_Diff_single
+                                       insert_absorb insert_ident)
+   apply clarsimp
+   apply (subgoal_tac "finite ys")
+    apply (simp add: sep.prod.remove)
+   apply (metis finite.insertI finite_image_iff)
+  apply (subgoal_tac "infinite ys", clarsimp)
+  using finite_image_iff by fastforce
+
+lemma add_mset_eq_mem:
+  "add_mset (P x) (image_mset P (mset_set F)) = image_mset Q (mset_set S')
+   \<Longrightarrow> \<exists>y. Q y = P x \<and> y \<in> S'"
+  apply (drule union_single_eq_member)
+  apply clarsimp
+  by (metis elem_mset_set empty_iff infinite_set_mset_mset_set)
+
+lemma sep_map_set_conj_mset_eq:
+  "\<lbrakk>image_mset P (mset_set S) = image_mset Q (mset_set S');
+    finite S; finite S'\<rbrakk>
+   \<Longrightarrow> sep_map_set_conj P S = sep_map_set_conj Q S'"
+  apply (induction S arbitrary: S' rule: infinite_finite_induct; clarsimp)
+   apply (simp add: mset_set_empty_iff)
+  apply (subgoal_tac "\<exists>y. y \<in> S' \<and> Q y = P x")
+   apply (clarsimp simp: sep.prod.remove mset_set.remove)
+  by (fastforce dest: union_single_eq_member)
+
+lemma sep_map_set_conj_multisetE:
+  "\<lbrakk>sep_map_set_conj P S s; finite S; finite S';
+    image_mset P (mset_set S) = image_mset Q (mset_set S')\<rbrakk>
+   \<Longrightarrow> sep_map_set_conj Q S' s"
+  by (subst sep_map_set_conj_mset_eq; fastforce)
+
+lemma not_in_image_vimage: "x \<notin> P ` S \<Longrightarrow> P -` {x} \<inter> S = {}"
+  by blast
+
+lemma bij_image_mset_eq:
+  "\<lbrakk>finite S; finite S'; P ` S = Q ` S';
+    (\<And>x. x \<in> P ` S \<Longrightarrow> \<exists>f. bij_betw f (P -` {x} \<inter> S) (Q -` {x} \<inter> S'))\<rbrakk>
+   \<Longrightarrow> image_mset P (mset_set S) = image_mset Q (mset_set S')"
+  apply (rule multiset_eqI)
+  apply (clarsimp simp: count_image_mset)
+  apply (case_tac "x \<in> Q ` S'"; clarsimp simp: bij_betw_iff_card not_in_image_vimage )
+  done
+
+lemma sep_map_set_elim:
+  "\<lbrakk>sep_map_set_conj P xs s;
+    xs = ys;
+    (\<And>x s. x \<in> xs \<Longrightarrow> P x s \<Longrightarrow> Q x s)\<rbrakk>
+   \<Longrightarrow> sep_map_set_conj Q ys s"
+  apply clarsimp
+  apply (case_tac "finite xs")
+   apply clarsimp
+   apply (erule sep_map_set_conj_impl)
+    apply atomize
+    apply (erule_tac x=x in allE)
+    apply clarsimp
+   apply clarsimp
+  apply clarsimp
+  done
+
+lemma sep_map_set_conj_Union:
+  "\<lbrakk>\<forall>s \<in> S. finite s;
+    \<forall>s s'. s \<in> S \<and> s' \<in> S \<longrightarrow> s \<noteq> s' \<longrightarrow> s \<inter> s' = {}\<rbrakk>
+   \<Longrightarrow> sep_map_set_conj (sep_map_set_conj P) S = sep_map_set_conj P (\<Union> S) "
+  apply (induct S rule: infinite_finite_induct; clarsimp)
+   apply (metis (no_types) finite_UnionD sep.prod.infinite)
+  apply (subst sep.prod.union_disjoint; clarsimp?)
+  by blast
+
+lemma sep_map_set_quotient_split:
+  "\<lbrakk>finite xs; equiv xs R\<rbrakk>
+   \<Longrightarrow> sep_map_set_conj P xs = sep_map_set_conj (sep_map_set_conj P ) (xs//R) "
+  apply (subst sep_map_set_conj_Union; clarsimp)
+    apply (meson in_quotient_imp_subset infinite_super)
+   apply (fastforce dest: quotient_disj)
+  by (simp add: Union_quotient)
+
+lemma sep_map_set_conj_congE:
+  "\<lbrakk>sep_map_set_conj (sep_map_set_conj P) xs s;
+    finite xs;
+    finite ys;
+    xs - {{}} = ys - {{}}\<rbrakk>
+   \<Longrightarrow> sep_map_set_conj (sep_map_set_conj P) ys s"
+  apply clarsimp
+  apply (induct xs arbitrary:ys s rule: infinite_finite_induct)
+    apply clarsimp+
+   apply (subgoal_tac "ys = {{}} \<or> ys = {}")
+    apply (erule disjE; clarsimp)
+   apply blast
+  apply clarsimp
+  apply (case_tac "x = {}")
+   apply (metis Diff_idemp Diff_insert_absorb Sep_Tactic_Helpers.sep_conj_empty sep.prod.empty)
+  apply (subgoal_tac "x \<in> ys")
+   apply (clarsimp simp: sep.prod.remove)
+   apply sep_cancel
+   apply (metis Diff_insert Diff_insert2 Diff_insert_absorb finite_Diff)
+  apply blast
+  done
+
+lemma sep_map_set_conj_cong_empty_eq:
+  "\<lbrakk>finite xs;
+    finite ys;
+    xs - {{}} = ys - {{}}\<rbrakk>
+   \<Longrightarrow> sep_map_set_conj (sep_map_set_conj P) xs = sep_map_set_conj (sep_map_set_conj P) ys "
+  apply clarsimp
+  apply (intro ext iffI; erule sep_map_set_conj_congE)
+  by blast+
+
+lemma sep_map_set_conj_match:
+  "sep_map_set_conj P S s \<Longrightarrow> (\<And>x s. x \<in> S \<Longrightarrow> P x s \<Longrightarrow> Q x s) \<Longrightarrow> sep_map_set_conj Q S s"
+  apply (induct rule: infinite_finite_induct; clarsimp)
+  apply (erule sep_conj_impl)
+   apply blast
+  by (metis sep_map_set_elim)
+
+lemma sep_map_set_squash:
+  "\<lbrakk>\<forall>x y. x \<in> S \<longrightarrow> y \<in> S \<longrightarrow> x \<noteq> y \<longrightarrow> f x = f y \<longrightarrow> f x = {}; finite S\<rbrakk>
+   \<Longrightarrow> sep_map_set_conj (\<lambda>v. sep_map_set_conj P (f v)) S =
+      sep_map_set_conj (sep_map_set_conj P) (f ` S)"
+  apply (induction S rule: infinite_finite_induct; clarsimp)
+  apply (case_tac "f x \<in> f ` F"; clarsimp)
+  apply (subgoal_tac "f x = {}")
+   apply clarsimp
+  apply blast
+  done
+
+lemma sep_map_set_conj_subst:
+  "(\<And>x. x \<in> S \<Longrightarrow> Q x = Q' x) \<Longrightarrow> sep_map_set_conj Q S = sep_map_set_conj Q' S"
+  by clarsimp
+
+lemma sep_map_zip_fst:
+  "(\<And>* map (\<lambda>(a,b). f a) (zip xs ys)) s =
+   (\<And>* map (\<lambda>a. f (fst a)) (zip xs ys)) s"
+  by (simp add: case_prod_unfold)
+
+lemma sep_map_zip_snd:
+  "(\<And>* map (\<lambda>(a, b). f b) (zip xs ys)) s =
+   (\<And>* map (\<lambda>a. f (snd a)) (zip xs ys)) s"
+  by (simp add: case_prod_unfold)
+
+declare sep_map_zip_fst[THEN iffD1, sep_cancel] sep_map_zip_fst[THEN iffD2, sep_cancel]
+        sep_map_zip_snd[THEN iffD1, sep_cancel] sep_map_zip_snd[THEN iffD2, sep_cancel]
+
+end
